Meta.v
@@ -23,77 +23,6 @@ Proof.
  intros H. f_equal. apply IH. omega with *. apply IH'. omega with *.
 Qed.
 
-(*
-Lemma freevars_fsubst v u t :
- ~Vars.In v (term_fvars t) -> term_fsubst v u t = t.
-Proof.
- revert t.
- fix IH 1. destruct t; simpl; trivial.
- - case eqbspec; trivial. intros <-. varsdec.
- - intros H. f_equal. clear f.
-   revert l H.
-   fix IH' 1. destruct l; simpl; trivial.
-   intros H. f_equal. apply IH. varsdec. apply IH'. varsdec.
-Qed.
-
-Lemma term_fsubst_bsubst v t n u T :
-  ~Vars.In v (term_fvars u) ->
-  term_closed t = true ->
-  term_fsubst v t (term_bsubst n u T) =
-  term_bsubst n u (term_fsubst v t T).
-Proof.
- revert T. fix IH 1. destruct T; simpl; intros.
- - case eqbspec; simpl; auto.
-   intros <-. now rewrite closed_bsubst.
- - case eqbspec; simpl; auto.
-   intros _. now apply freevars_fsubst.
- - f_equal. clear f.
-   revert l. fix IH' 1. destruct l; simpl; trivial.
-   f_equal. now apply IH. now apply IH'.
-Qed.
-
-Lemma fsubst_bsubst v t n u f :
-  ~Vars.In v (term_fvars u) ->
-  term_closed t = true ->
-  form_fsubst v t (form_bsubst n u f) =
-  form_bsubst n u (form_fsubst v t f).
-Proof.
- revert n.
- induction f; simpl; intros; f_equal; auto.
- injection (term_fsubst_bsubst v t n u (Fun "" l)); auto.
-Qed.
-*)
-
-Definition subinvars (sub : subst) :=
-  vars_unionmap (fun '(v,_) => Vars.singleton v) sub.
-
-Definition suboutvars (sub : subst) :=
-  vars_unionmap (fun '(_,t) => fvars t) sub.
-
-Definition subvars (sub : subst) :=
-  Vars.union (subinvars sub) (suboutvars sub).
-
-Definition sub_closed (sub : subst) :=
-  forallb (fun '(_,t) => term_closed t) sub.
-
-Lemma subinvars_in sub (z:variable) :
- Vars.In z (subinvars sub) <-> In z (map fst sub).
-Proof.
- induction sub as [|(a,u) sub IH]; simpl;
-  rewrite <- ?IH; auto with sets.
-Qed.
-
-Lemma list_assoc_suboutvars sub t v :
- list_assoc v sub = Some t ->
- Vars.Subset (term_fvars t) (suboutvars sub).
-Proof.
- induction sub as [|(x,u) sub IH]; simpl.
- - easy.
- - case eqbspec.
-   + intros <- [= ->]. varsdec.
-   + intros NE H. specialize (IH H). varsdec.
-Qed.
-
 Lemma term_vmap_ext h h' (t:term) :
  (forall v:variable, Vars.In v (fvars t) -> h v = h' v) ->
  term_vmap h t = term_vmap h' t.
@@ -103,6 +32,22 @@ Proof.
  - auto with sets.
  - f_equal. clear f. revert l E.
    fix IH' 1; destruct l; cbn; intros; f_equal; auto with sets.
+Qed.
+
+Lemma form_vmap_ext h h' (f:formula) :
+ (forall v:variable, Vars.In v (fvars f) -> h v = h' v) ->
+ form_vmap h f = form_vmap h' f.
+Proof.
+ induction f; cbn; intro; f_equal; auto with sets.
+ now injection (term_vmap_ext h h' (Fun "" l)).
+Qed.
+
+Lemma ctx_vmap_ext h h' (c:context) :
+ (forall v:variable, Vars.In v (fvars c) -> h v = h' v) ->
+ ctx_vmap h c = ctx_vmap h' c.
+Proof.
+ induction c; cbn; intros; f_equal;
+  auto using form_vmap_ext with sets.
 Qed.
 
 Lemma term_vmap_id h (t:term) :
@@ -116,46 +61,12 @@ Proof.
    fix IH' 1; destruct l; cbn; intros; f_equal; auto with sets.
 Qed.
 
-Lemma term_vmap_vmap h h' (t:term) :
- term_vmap h (term_vmap h' t) =
- term_vmap (fun v => term_vmap h (h' v)) t.
-Proof.
- revert t.
- fix IH 1; destruct t; simpl; trivial.
- f_equal. clear f. revert l.
- fix IH' 1; destruct l; simpl; f_equal; auto.
-Qed.
-
-Lemma form_vmap_ext h h' (f:formula) :
- (forall v:variable, Vars.In v (fvars f) -> h v = h' v) ->
- form_vmap h f = form_vmap h' f.
-Proof.
- induction f; cbn; intro; f_equal; auto with sets.
- now injection (term_vmap_ext h h' (Fun "" l)).
-Qed.
-
 Lemma form_vmap_id h (f:formula) :
  (forall v:variable, Vars.In v (fvars f) -> h v = FVar v) ->
  form_vmap h f = f.
 Proof.
  induction f; cbn; intro; f_equal; auto with sets.
  now injection (term_vmap_id h (Fun "" l)).
-Qed.
-
-Lemma form_vmap_vmap h h' (f:formula) :
- form_vmap h (form_vmap h' f) =
- form_vmap (fun v => term_vmap h (h' v)) f.
-Proof.
- induction f; cbn; f_equal; auto.
- now injection (term_vmap_vmap h h' (Fun "" l)).
-Qed.
-
-Lemma ctx_vmap_ext h h' (c:context) :
- (forall v:variable, Vars.In v (fvars c) -> h v = h' v) ->
- ctx_vmap h c = ctx_vmap h' c.
-Proof.
- induction c; cbn; intros; f_equal;
-  auto using form_vmap_ext with sets.
 Qed.
 
 Lemma ctx_vmap_id h (c:context) :
@@ -166,6 +77,24 @@ Proof.
   auto using form_vmap_id with sets.
 Qed.
 
+Lemma term_vmap_vmap h h' (t:term) :
+ term_vmap h (term_vmap h' t) =
+ term_vmap (fun v => term_vmap h (h' v)) t.
+Proof.
+ revert t.
+ fix IH 1; destruct t; simpl; trivial.
+ f_equal. clear f. revert l.
+ fix IH' 1; destruct l; simpl; f_equal; auto.
+Qed.
+
+Lemma form_vmap_vmap h h' (f:formula) :
+ form_vmap h (form_vmap h' f) =
+ form_vmap (fun v => term_vmap h (h' v)) f.
+Proof.
+ induction f; cbn; f_equal; auto.
+ now injection (term_vmap_vmap h h' (Fun "" l)).
+Qed.
+
 Lemma ctx_vmap_vmap h h' (c:context) :
  ctx_vmap h (ctx_vmap h' c) =
  ctx_vmap (fun v => term_vmap h (h' v)) c.
@@ -173,219 +102,151 @@ Proof.
  induction c; cbn; f_equal; auto using form_vmap_vmap with sets.
 Qed.
 
-Lemma ctx_fsubsts_alt sub c :
- ctx_fsubsts sub c = ctx_vmap (fsubsts sub) c.
-Proof.
- reflexivity.
-Qed.
+Arguments Vars.union !_ !_.
 
-(*
-Lemma term_fvars_vmap h t :
+Lemma term_fvars_vmap h (t:term) :
   Vars.Subset
-    (term_fvars (term_vmap h t))
-    (vars_flatmap (fun v => term_fvars (h v))
-                  (Vars.elements (term_fvars t))).
-Proof.
- revert t.
- fix IH 1. destruct t; simpl.
- - varsdec.
- - varsdec.
- - clear f. revert l. fix IH' 1. destruct l; simpl.
-   + varsdec.
-   + specialize (IH t). specialize (IH' l). varsdec.
-*)
-
-Lemma term_fvars_fsubsts sub (t:term) :
-  Vars.Subset
-    (fvars (term_fsubsts sub t))
-    (Vars.union (suboutvars sub)
-                (Vars.diff (fvars t) (subinvars sub))).
+    (fvars (term_vmap h t))
+    (vars_flatmap (fun v => fvars (h v)) (fvars t)).
 Proof.
  revert t.
  fix IH 1. destruct t; cbn.
- - unfold fsubsts. rewrite ?list_assoc_dft_alt.
-   destruct (list_assoc v sub) eqn:E; cbn.
-   + apply list_assoc_suboutvars in E. varsdec.
-   + rewrite list_assoc_notin, <- subinvars_in in E. varsdec.
+ - varsdec.
  - varsdec.
  - clear f. revert l. fix IH' 1. destruct l; cbn.
    + varsdec.
-   + specialize (IH t). specialize (IH' l). varsdec.
+   + specialize (IH t). specialize (IH' l).
+     rewrite vars_flatmap_union. varsdec.
 Qed.
 
-Lemma fvars_fsubsts sub (f:formula) :
+Lemma form_fvars_vmap h (f:formula) :
   Vars.Subset
-    (fvars (form_fsubsts sub f))
-    (Vars.union (suboutvars sub)
-                (Vars.diff (fvars f) (subinvars sub))).
+    (fvars (form_vmap h f))
+    (vars_flatmap (fun v => fvars (h v)) (fvars f)).
 Proof.
- induction f; cbn; auto; try varsdec.
- apply (term_fvars_fsubsts sub (Fun "" l)).
+ induction f; cbn; try varsdec.
+ - apply (term_fvars_vmap h (Fun "" l)).
+ - rewrite vars_flatmap_union. varsdec.
 Qed.
 
-Lemma fvars_fsubsts_ctx sub (c:context) :
+Lemma ctx_fvars_vmap h (c:context) :
   Vars.Subset
-    (fvars (ctx_fsubsts sub c))
-    (Vars.union (suboutvars sub)
-                (Vars.diff (fvars c) (subinvars sub))).
+    (fvars (ctx_vmap h c))
+    (vars_flatmap (fun v => fvars (h v)) (fvars c)).
 Proof.
  induction c as [|f c IH]; cbn.
  - varsdec.
- - generalize (fvars_fsubsts sub f). varsdec.
+ - generalize (form_fvars_vmap h f).
+   rewrite vars_flatmap_union. varsdec.
 Qed.
 
-Lemma fvars_fsubsts_seq sub (s:sequent) :
+Lemma seq_fvars_vmap h (s:sequent) :
   Vars.Subset
-    (fvars (seq_fsubsts sub s))
-    (Vars.union (suboutvars sub)
-                (Vars.diff (fvars s) (subinvars sub))).
+    (fvars (seq_vmap h s))
+    (vars_flatmap (fun v => fvars (h v)) (fvars s)).
 Proof.
- destruct s as (c,f). cbn.
- generalize (fvars_fsubsts_ctx sub c) (fvars_fsubsts sub f).
- varsdec.
+ destruct s. cbn.
+ rewrite vars_flatmap_union.
+ generalize (form_fvars_vmap h f) (ctx_fvars_vmap h c). varsdec.
 Qed.
 
-Lemma term_fsubsts_notIn sub (x:variable) u t :
- ~Vars.In x (fvars t) ->
- term_fsubsts ((x, u) :: sub) t = term_fsubsts sub t.
-Proof.
- intros NI. apply term_vmap_ext.
- intros v IN. unfold fsubsts. rewrite !list_assoc_dft_alt.
- simpl. case eqbspec; auto with sets.
-Qed.
-
-Lemma form_fsubsts_notIn sub (x:variable) u f :
- ~Vars.In x (fvars f) ->
- form_fsubsts ((x, u) :: sub) f = form_fsubsts sub f.
-Proof.
- intros NI. apply form_vmap_ext.
- intros v IN. unfold fsubsts. rewrite !list_assoc_dft_alt.
- simpl. case eqbspec; auto with sets.
-Qed.
-
-Lemma ctx_fsubsts_notIn sub (x:variable) u c :
- ~Vars.In x (fvars c) ->
- ctx_fsubsts ((x,u)::sub) c = ctx_fsubsts sub c.
-Proof.
- intros NI. apply ctx_vmap_ext.
- intros v IN. unfold fsubsts. rewrite !list_assoc_dft_alt.
- simpl. case eqbspec; auto with sets.
-Qed.
-
-Lemma term_fsubsts_nop sub t :
- Vars.Empty (Vars.inter (subinvars sub) (fvars t)) ->
- term_fsubsts sub t = t.
-Proof.
- intros E. apply term_vmap_id.
- intros v Hv. unfold fsubsts. rewrite list_assoc_dft_alt.
- assert (H : ~Vars.In v (subinvars sub)) by varsdec.
- rewrite subinvars_in, <- list_assoc_notin in H.
- now rewrite H.
-Qed.
-
-Lemma form_fsubsts_nop sub f :
- Vars.Empty (Vars.inter (subinvars sub) (fvars f)) ->
- form_fsubsts sub f = f.
-Proof.
- intros E. apply form_vmap_id.
- intros v Hv. unfold fsubsts. rewrite list_assoc_dft_alt.
- assert (H : ~Vars.In v (subinvars sub)) by varsdec.
- rewrite subinvars_in, <- list_assoc_notin in H.
- now rewrite H.
-Qed.
-
-Lemma ctx_fsubsts_nop sub c:
- Vars.Empty (Vars.inter (subinvars sub) (fvars c)) ->
- ctx_fsubsts sub c = c.
-Proof.
- intros E. apply ctx_vmap_id.
- intros v Hv. unfold fsubsts. rewrite list_assoc_dft_alt.
- assert (H : ~Vars.In v (subinvars sub)) by varsdec.
- rewrite subinvars_in, <- list_assoc_notin in H.
- now rewrite H.
-Qed.
-
-Lemma term_fsubsts_bsubst sub n u t :
- sub_closed sub = true ->
- term_fsubsts sub (term_bsubst n u t) =
-  term_bsubst n (term_fsubsts sub u) (term_fsubsts sub t).
+Lemma term_vmap_bsubst h n u t :
+ (forall v, term_closed (h v) = true) ->
+ term_vmap h (term_bsubst n u t) =
+  term_bsubst n (term_vmap h u) (term_vmap h t).
 Proof.
  intros CL.
  revert t.
- fix IH 1. destruct t; simpl; auto.
- - unfold fsubsts; rewrite list_assoc_dft_alt.
-   destruct (list_assoc v sub) eqn:E; simpl; auto.
-   symmetry. apply closed_bsubst.
-   apply list_assoc_in2 in E.
-   unfold sub_closed in CL. rewrite forallb_forall in CL.
-   now apply (CL (v,t)).
+ fix IH 1. destruct t; cbn.
+ - symmetry. apply closed_bsubst. apply CL.
  - case eqbspec; simpl; auto.
  - f_equal. clear f.
    revert l. fix IH' 1. destruct l; simpl; auto.
    f_equal. apply IH. apply IH'.
 Qed.
 
-Lemma fsubsts_bsubst sub n u A :
- sub_closed sub = true ->
- form_fsubsts sub (form_bsubst n u A) =
-  form_bsubst n (term_fsubsts sub u) (form_fsubsts sub A).
+Lemma form_vmap_bsubst h n u f :
+ (forall v, term_closed (h v) = true) ->
+ form_vmap h (form_bsubst n u f) =
+  form_bsubst n (term_vmap h u) (form_vmap h f).
 Proof.
  intros CL. revert n.
- induction A; simpl; intros n; f_equal; auto.
- injection (term_fsubsts_bsubst sub n u (Fun "" l)); auto.
+ induction f; cbn; intros n; f_equal; auto.
+ injection (term_vmap_bsubst h n u (Fun "" l)); auto.
 Qed.
 
-Lemma fsubsts_bsubst_adhoc sub x t f :
- sub_closed ((x,t)::sub) = true ->
+Lemma vmap_bsubst_adhoc h x t f :
+ (forall v, term_closed (h v) = true) ->
+ term_closed t = true ->
  ~Vars.In x (fvars f) ->
- form_fsubsts ((x,t)::sub) (form_bsubst 0 (FVar x) f) =
- form_bsubst 0 t (form_fsubsts sub f).
+ form_vmap (fun v => if v =? x then t else h v)
+   (form_bsubst 0 (FVar x) f) =
+ form_bsubst 0 t (form_vmap h f).
 Proof.
  intros.
- rewrite fsubsts_bsubst by trivial.
- simpl. unfold fsubsts. rewrite list_assoc_dft_alt. simpl.
- rewrite eqb_refl.
- f_equal.
- now apply form_fsubsts_notIn.
+ rewrite form_vmap_bsubst.
+ - simpl. rewrite eqb_refl. f_equal.
+   apply form_vmap_ext.
+   intros v Hv. case eqbspec; auto with sets.
+ - intros v. case eqbspec; auto.
 Qed.
 
-Lemma Pr_fsubsts logic s :
+Lemma Pr_vmap logic s :
   Pr logic s ->
-  forall sub, sub_closed sub = true ->
-  Pr logic (seq_fsubsts sub s).
+  forall h, (forall v, term_closed (h v) = true) ->
+  Pr logic (seq_vmap h s).
 Proof.
  induction 1; cbn in *; intros; auto.
  - apply R_Ax. now apply in_map.
- - apply R_Not_e with (form_fsubsts sub A); auto.
- - apply R_And_e1 with (form_fsubsts sub B); auto.
- - apply R_And_e2 with (form_fsubsts sub A); auto.
- - apply R_Or_e with (form_fsubsts sub A) (form_fsubsts sub B); auto.
- - apply R_Imp_e with (form_fsubsts sub A); auto.
- - set (vars := Vars.union (fvars (Γ⊢A)) (subvars sub)).
+ - apply R_Not_e with (form_vmap h A); auto.
+ - apply R_And_e1 with (form_vmap h B); auto.
+ - apply R_And_e2 with (form_vmap h A); auto.
+ - apply R_Or_e with (form_vmap h A) (form_vmap h B); auto.
+ - apply R_Imp_e with (form_vmap h A); auto.
+ - set (vars := Vars.union (fvars (Γ⊢A))
+                  (vars_flatmap (fun v => fvars (h v)) (fvars (Γ⊢A)))).
    set (z := fresh_var vars).
    apply R_All_i with z.
-   + intros H'. apply (fvars_fsubsts_seq sub (Γ⊢A)) in H'.
-     apply (fresh_var_ok vars). unfold subvars in vars. varsdec.
-   + specialize (IHPr ((x,FVar z)::sub)).
-     rewrite ctx_fsubsts_notIn in IHPr by varsdec.
-     rewrite <- fsubsts_bsubst_adhoc with (x:=x); auto with sets.
- - rewrite fsubsts_bsubst by auto.
+   + intros H'. apply (seq_fvars_vmap h (Γ⊢A)) in H'.
+     apply (fresh_var_ok vars). varsdec.
+   + specialize (IHPr (fun v => if v =? x then FVar z else h v)).
+     rewrite <- (ctx_vmap_ext h) in IHPr by
+       (intros; case eqbspec; auto with sets).
+     rewrite <- vmap_bsubst_adhoc with (x:=x); auto with sets.
+     apply IHPr.
+     intros v; case eqbspec; auto.
+ - rewrite form_vmap_bsubst by auto.
    apply R_All_e; auto.
- - specialize (IHPr sub).
-   rewrite fsubsts_bsubst in IHPr by auto.
-   apply R_Ex_i with (term_fsubsts sub t); auto.
- - set (vars := Vars.union (fvars (A::Γ⊢B)) (subvars sub)).
+ - specialize (IHPr h).
+   rewrite form_vmap_bsubst in IHPr by auto.
+   apply R_Ex_i with (term_vmap h t); auto.
+ - set (vars := Vars.union (fvars (A::Γ⊢B))
+                 (vars_flatmap (fun v => fvars (h v)) (fvars (A::Γ⊢B)))).
    set (z := fresh_var vars).
-   apply R_Ex_e with z (form_fsubsts sub A).
-   + intros H'. apply (fvars_fsubsts_seq sub (A::Γ⊢B) z) in H'.
-     apply (fresh_var_ok vars). unfold subvars in vars. varsdec.
+   apply R_Ex_e with z (form_vmap h A).
+   + intros H'. apply (seq_fvars_vmap h (A::Γ⊢B) z) in H'.
+     apply (fresh_var_ok vars). varsdec.
    + now apply IHPr1.
-   + specialize (IHPr2 ((x,FVar z)::sub)).
-     rewrite ctx_fsubsts_notIn in IHPr2 by varsdec.
-     rewrite fsubsts_bsubst_adhoc in IHPr2; auto; try varsdec.
-     rewrite form_fsubsts_notIn in IHPr2 by varsdec.
-     auto.
+   + specialize (IHPr2 (fun v => if v =? x then FVar z else h v)).
+     rewrite <- (ctx_vmap_ext h) in IHPr2 by
+       (intros; case eqbspec; auto with sets).
+     rewrite <- (form_vmap_ext h _ B) in IHPr2 by
+       (intros; case eqbspec; auto with sets).
+     rewrite <- vmap_bsubst_adhoc with (x:=x); auto with sets.
+     apply IHPr2.
+     intros v; case eqbspec; auto.
  - apply R_Absu with l. auto.
+Qed.
+
+Lemma Pr_fsubst logic s :
+  Pr logic s ->
+  forall v t, term_closed t = true ->
+  Pr logic (seq_fsubst v t s).
+Proof.
+ intros.
+ change (seq_fsubst v t) with (seq_vmap (fsubst v t)).
+ apply Pr_vmap; auto.
+ intros x. unfold fsubst. case eqbspec; auto.
 Qed.
 
 Definition ListSubset {A} (l l': list A) :=
@@ -418,7 +279,7 @@ Lemma Pr_weakening logic s s' :
 Proof.
  intros H. revert s'.
  induction H; inversion_clear 1; auto.
- - apply R_Not_e with A; auto.
+ - eapply R_Not_e with A; auto.
  - apply R_And_e1 with B; auto.
  - apply R_And_e2 with A; auto.
  - apply R_Or_e with A B; auto.
@@ -427,58 +288,54 @@ Proof.
    set (z := fresh_var vars).
    assert (Hz : ~Vars.In z vars) by (apply fresh_var_ok).
    clearbody z; unfold vars in *; clear vars.
-   set (Γ2 := ctx_fsubsts [(x,FVar z)] Γ').
+   set (h := fun v => if v =? x then FVar z else FVar v).
+   set (Γ2 := ctx_vmap h Γ').
    assert (~Vars.In x (fvars Γ2)).
-   { intros IN. apply fvars_fsubsts_ctx in IN. varsdec'. }
+   { intros IN. apply ctx_fvars_vmap in IN.
+     rewrite vars_flatmap_in in IN.
+     destruct IN as (v & IN & IN'). revert IN.
+     unfold h. case eqbspec; cbn; varsdec. }
+   assert (ListSubset Γ Γ2).
+   { rewrite <- (ctx_vmap_id h Γ).
+     now apply ListSubset_map.
+     intros v Hv. unfold h. case eqbspec; auto. varsdec'. }
    assert (PR : Pr l (Γ2 ⊢ ∀A)).
-   { apply R_All_i with x.
-     - varsdec'.
-     - apply IHPr. clear IHPr. constructor.
-       rewrite <- (ctx_fsubsts_nop [(x, FVar z)] Γ) by varsdec'.
-       now apply ListSubset_map. }
-   apply Pr_fsubsts with (sub:=[(z,FVar x)]) in PR; auto.
-   simpl in PR.
-   assert (E : ctx_fsubsts [(z, FVar x)] Γ2 = Γ').
-   { unfold Γ2.
-     rewrite !ctx_fsubsts_alt.
-     rewrite ctx_vmap_vmap. apply ctx_vmap_id.
-     intros v IN. unfold fsubsts. simpl.
-     case eqbspec; simpl; case eqbspec; intros; subst; auto.
-     easy.
-     varsdec'. }
-   rewrite E in PR.
-   rewrite form_fsubsts_nop in PR by varsdec'.
-   trivial.
+   { apply R_All_i with x; auto. varsdec'. }
+   set (h' := fun v => if v =? z then FVar x else FVar v).
+   assert (forall v, term_closed (h' v) = true).
+   { intros v. unfold h'. case eqbspec; now cbn. }
+   apply Pr_vmap with (h := h') in PR; auto.
+   simpl in PR. unfold Γ2 in PR.
+   rewrite ctx_vmap_vmap, ctx_vmap_id, form_vmap_id in PR; auto.
+   + intros v hv. unfold h'. case eqbspec; auto. varsdec'.
+   + intros v hv. unfold h, h'.
+     do 2 (case eqbspec; cbn); intros; subst; try easy. varsdec'.
  - apply R_Ex_i with t; auto.
  - set (vars := Vars.add x (fvars (A::Γ' ⊢ B))).
    set (z := fresh_var vars).
    assert (Hz : ~Vars.In z vars) by (apply fresh_var_ok).
    clearbody z; unfold vars in *; clear vars.
-   set (Γ2 := ctx_fsubsts [(x,FVar z)] Γ').
+   set (h := fun v => if v =? x then FVar z else FVar v).
+   set (Γ2 := ctx_vmap h Γ').
    assert (~Vars.In x (fvars Γ2)).
-   { intros IN. apply fvars_fsubsts_ctx in IN. varsdec'. }
+   { intros IN. apply ctx_fvars_vmap in IN.
+     rewrite vars_flatmap_in in IN.
+     destruct IN as (v & IN & IN'). revert IN.
+     unfold h. case eqbspec; cbn; varsdec. }
+   assert (ListSubset Γ Γ2).
+   { rewrite <- (ctx_vmap_id h Γ).
+     now apply ListSubset_map.
+     intros v Hv. unfold h. case eqbspec; auto. varsdec'. }
    assert (PR : Pr l (Γ2 ⊢ B)).
-   { apply R_Ex_e with x A.
-     - varsdec'.
-     - apply IHPr1. clear IHPr1 IHPr2. constructor.
-       rewrite <- (ctx_fsubsts_nop [(x, FVar z)] Γ) by varsdec'.
-       now apply ListSubset_map.
-     - apply IHPr2. clear IHPr1 IHPr2. constructor.
-       apply ListSubset_cons.
-       rewrite <- (ctx_fsubsts_nop [(x, FVar z)] Γ) by varsdec'.
-       now apply ListSubset_map. }
-   apply Pr_fsubsts with (sub:=[(z,FVar x)]) in PR; auto.
-   simpl in PR.
-   assert (E : ctx_fsubsts [(z, FVar x)] Γ2 = Γ').
-   { unfold Γ2.
-     rewrite !ctx_fsubsts_alt.
-     rewrite ctx_vmap_vmap. apply ctx_vmap_id.
-     intros v IN. unfold fsubsts. simpl.
-     case eqbspec; simpl; case eqbspec; intros; subst; auto.
-     easy.
-     varsdec'. }
-   rewrite E in PR.
-   rewrite form_fsubsts_nop in PR by varsdec'.
-   trivial.
+   { apply R_Ex_e with x A; auto. varsdec'. }
+   set (h' := fun v => if v =? z then FVar x else FVar v).
+   assert (forall v, term_closed (h' v) = true).
+   { intros v. unfold h'. case eqbspec; now cbn. }
+   apply Pr_vmap with (h := h') in PR; auto.
+   simpl in PR. unfold Γ2 in PR.
+   rewrite ctx_vmap_vmap, ctx_vmap_id, form_vmap_id in PR; auto.
+   + intros v hv. unfold h'. case eqbspec; auto. varsdec'.
+   + intros v hv. unfold h, h'.
+     do 2 (case eqbspec; cbn); intros; subst; try easy. varsdec'.
  - apply R_Absu with l; auto.
 Qed.
